LeanPy/Data/NonScalarRef.lean
@@ -1,0 +1,58 @@
+/-
+Copyright (c) 2025 Mac Malone. All rights reserved.
+Released under the Apache 2.0 license as described in the file LICENSE.
+syntax Authors Mac Malone
+-/
+import LeanPy.Util.WithAddr
+
+namespace LeanPy
+
+structure NonScalarRef (α : Type u) where
+  toWithAddr : WithAddr α
+  wf : toWithAddr.addr % 2 = 0
+
+namespace NonScalarRef
+
+@[inline] def addr (n : NonScalarRef α) : USize :=
+  n.toWithAddr.addr
+
+@[simp] theorem addr_mk : addr (mk a h) = a.addr := rfl
+
+@[simp] theorem addr_mod_two : addr a % 2 = 0 := a.wf
+
+@[simp] theorem toNat_addr_mod_two : (addr a).toNat % 2 = 0 := by
+  simpa [← USize.toNat_inj, -addr_mod_two] using addr_mod_two
+
+@[inline] def data (n : NonScalarRef α) : α :=
+  n.toWithAddr.data
+
+@[simp] theorem data_mk : data (mk a h) = a.data := rfl
+
+instance : CoeOut (NonScalarRef α) α := ⟨data⟩
+
+private noncomputable def null (a : α) : NonScalarRef α :=
+  ⟨.mk 0 a, by simp⟩
+
+@[simp] private theorem data_null : data (null a) = a := rfl
+
+instance [Nonempty α] : Nonempty (NonScalarRef α) :=
+  ⟨null Classical.ofNonempty⟩
+
+end NonScalarRef
+
+/-! ## StringRef -/
+
+abbrev StringRef := NonScalarRef String
+
+deriving instance TypeName for StringRef
+
+@[inline] private unsafe def mkStringRefImpl
+  (s : String) : BaseIO {r : StringRef // r.data = s}
+:= pure (unsafeCast s)
+
+@[implemented_by mkStringRefImpl]
+opaque mkStringRef' (s : String) : BaseIO {r : StringRef // r.data = s} :=
+  pure ⟨NonScalarRef.null s, NonScalarRef.data_null⟩
+
+@[inline] def mkStringRef (s : String) : BaseIO StringRef := do
+  Subtype.val <$> mkStringRef' s
