LeanPy/Data/Object/Basic.lean
@@ -239,6 +239,77 @@ instance : CoeDep (Option α) none Object := ⟨.none⟩
 
 @[simp] theorem Object.isNone_none : isNone none := rfl
 
+/-! ## `str` Objects -/
+
+def strRepr (s : String) : String :=
+  let q := if s.contains '\'' && !s.contains '"' then '"' else '\''
+  go s q 0 ("".push q) |>.push q
+where
+  go s q p ns : String :=
+    if h : s.atEnd p then
+      ns
+    else
+      let c := s.get' p h
+      let p' := s.next' p h
+      if c == q then
+        go s q p' (ns.push '\\' |>.push q)
+      else if c == '\\' then
+        go s q p' (ns.push '\\' |>.push '\\')
+      else if c == '\t' then
+        go s q p' (ns.push '\\' |>.push 't')
+      else if c == '\r' then
+        go s q p' (ns.push '\\' |>.push 'r')
+      else if c == '\n' then
+        go s q p' (ns.push '\\' |>.push 'n')
+      else if c.val < 0x20 || c.val == 0x7f then
+        go s q p' (upperHexUInt8 c.val.toUInt8 (ns.push '\\' |>.push 'x'))
+      else if c.val < 0x7f || isPrintableUnicode c then
+        go s q p' (ns.push c)
+      else if c.val < 0x100 then
+        go s q p' (upperHexUInt8 c.val.toUInt8 (ns.push '\\' |>.push 'x'))
+      else if c.val < 0x10000 then
+        go s q p' (upperHexUInt16 c.val.toUInt16 (ns.push '\\' |>.push 'u'))
+      else
+        go s q p' (upperHexUInt32 c.val (ns.push '\\' |>.push 'U'))
+  termination_by s.utf8ByteSize - p.byteIdx
+  decreasing_by all_goals
+    apply Nat.sub_lt_sub_left
+    · simpa [String.atEnd] using h
+    · exact String.lt_next' ..
+  @[inline] isPrintableUnicode c :=
+    -- TODO: Use unicode definition once Lean has support for it
+    Lean.isLetterLike c
+
+def strTypeSlots : DTypeSlots StringRef where
+  bool self := return self.data.data.length != 0
+  str self := return self.data.data
+  repr self := return strRepr self.data.data
+
+initialize strTypeSlotsRef : DTypeSlotsRef StringRef ←
+  mkDTypeSlotsRef strTypeSlots
+
+def strType : DTypeObject StringRef where
+  name := "str"
+  doc? := some "\
+    str(object='') -> str\n\
+    str(bytes_or_buffer[, encoding[, errors]]) -> str\n\
+    \n\
+    Create a new string object from the given object. If encoding or\n\
+    errors is specified, then the object must expose a data buffer\n\
+    that will be decoded using the given encoding and error handler.\n\
+    Otherwise, returns the result of object.__str__() (if defined)\n\
+    or repr(object).\n\
+    encoding defaults to sys.getdefaultencoding().\n\
+    errors defaults to 'strict'.
+  "
+  slots := strTypeSlotsRef
+
+@[inline] def Object.ofStringRef (r : StringRef) : Object :=
+  .mk strType r r.id
+
+@[inline] def mkStringObject (s : String) : BaseIO Object := do
+  Object.ofStringRef <$> mkStringRef s
+
 /-! ## `int` Objects -/
 
 def intTypeSlots : DTypeSlots IntRef where
